
\documentclass[12pt]{article}
\usepackage{amsmath, amssymb}
\usepackage[margin=1in]{geometry}
\title{Assignment Sheet 1\\ \large MA2020 Differential Equations (July - November 2012)}
\date{}

\begin{document}
\maketitle

\section*{1. Solve the following first order differential equations}

\begin{enumerate}
  \item[(a)] $ x \frac{dy}{dx} + y = x^3 y^6 $
  \item[(b)] $ x y^2 \frac{dy}{dx} + y^3 = x \cos(x) $
  \item[(c)] $ x \frac{dy}{dx} + y = y^2 \log(x) $
  \item[(d)] $ (x^2 y^3 + x y) \frac{dy}{dx} = 1 $
  \item[(e)] $ \frac{dy}{dx} + (2x \tan^{-1} y - x^3)(1 + y^2) = 0 $
  \item[(f)] $ (x^2 + y)dx + (y^3 + x)dy = 0 $
  \item[(g)] $ (1 + e^{x/y})dx + e^{x/y}\left(1 - \frac{x}{y}\right)dy = 0 $
  \item[(h)] $ (y^2 e^{x y^2} + 4x^3)dx + (2x y e^{x y^2} - 3y^2)dy = 0 $
  \item[(i)] $ (x\,dx + y\,dy)(x^2 + y^2) = y\,dx - x\,dy $
  \item[(j)] $ y \cos(x)dx + 2 \sin(x)dy = 0 $
  \item[(k)] $ x\,dy + y\,dx + 3x^3 y^4 dy = 0 $
  \item[(l)] $ (1 + xy)y\,dx + (1 - xy)x\,dy = 0 $
  \item[(m)] $ (y^4 + 2y)dx + (x y^3 + 2y^4 - 4x)dy = 0 $
  \item[(n)] $ (xy - 1)dx + (x^2 - xy)dy = 0 $
\end{enumerate}

\section*{2.}
Find the curve passing through the point (1, 0) and having at each of its points the slope $ -\frac{x}{y} $

\section*{3. Solve the following Initial Value Problems (IVP)}

\begin{enumerate}
  \item[(a)] $ \frac{dy}{dx} = 2y + e^{2x}, \quad y(0) = 3 $
  \item[(b)] $ \frac{dy}{dx} = 3y + 2e^{3x}, \quad y(0) = 2 $
  \item[(c)] $ \frac{dy}{dx} = y \tan(x) + \sec(x), \quad y(0) = -1 $
  \item[(d)] $ \frac{dy}{dx} = \frac{2}{x}y + x, \quad y(1) = 2 $
\end{enumerate}

\section*{4.}
Define the Wronskian $ w(y_1, y_2) $ of any two continuous functions $ y_1 $ and $ y_2 $ defined in an interval $ (a, b) \subset \mathbb{R} $. Show that $ w(y_1, y_2) = 0 $ if $ y_1 $ and $ y_2 $ are linearly dependent.

\section*{5.}
If $ y_1 $ and $ y_2 $ are any two solutions of a second order linear homogeneous ordinary differential equation defined in an interval $ (a, b) \subset \mathbb{R} $, then $ w(y_1, y_2) $ is either identically zero or non-zero at any point of the interval.

\section*{6.}
If $ y_1 $ and $ y_2 $ are two linearly independent solutions of a second order linear homogeneous ODE, then prove that $ y = c_1 y_1 + c_2 y_2 $, where $ c_1 $ and $ c_2 $ are constants, is a general solution.

\section*{7. Find the general solution of the following second order equations using the given known solution $ y_1 $}

\begin{enumerate}
  \item[(a)] $ x^2 \frac{d^2 y}{dx^2} + x \frac{dy}{dx} - y = 0 \quad \text{where } y_1(x) = x $
  \item[(b)] $ x^2 \frac{d^2 y}{dx^2} + x \frac{dy}{dx} - 4y = 0 \quad \text{where } y_1(x) = x^2 $
  \item[(c)] $ (x - 1) \frac{d^2 y}{dx^2} - x \frac{dy}{dx} + y = 0 \quad \text{where } y_1(x) = x $
  \item[(d)] $ x \frac{d^2 y}{dx^2} - (2x + 1) \frac{dy}{dx} + (x + 1)y = 0 \quad \text{where } y_1(x) = e^x $
\end{enumerate}

\section*{8. Find the general solution of each of the following equations ($ D^n \equiv \frac{d^n}{dx^n} $)}

\begin{enumerate}
  \item[(a)] $ (D^4 - 81)y = 0 $
  \item[(b)] $ (D^3 - 4D^2 + 5D - 2)y = 0 $
  \item[(c)] $ (D^4 - 7D^3 + 18D^2 - 20D + 8)y = 0 $
  \item[(d)] $ (D^4 + 2D^3 + 3D^2 + 2D + 1)y = 0 $
  \item[(e)] $ (D^2 - 3D - 6)y = 3 \sin 2x $
  \item[(f)] $ (D^2 + 1)y = 2 \cos x $
  \item[(g)] $ (D^2 - 3D + 2)y = (4x + 5)e^{3x} $
  \item[(h)] $ (D^2 - 1)y = 3e^{2x} \cos 2x $
  \item[(i)] $ (D^2 - 2D + 3)y = 3e^{-x} \cos x $
\end{enumerate}

\section*{9. Solve using the method of variation of parameters ($ D^n \equiv \frac{d^n}{dx^n} $)}

\begin{enumerate}
  \item[(a)] $ (D^2 + 1)y = \csc x $
  \item[(b)] $ (D^2 - D - 6)y = e^{-x} $
  \item[(c)] $ (D^2 + a^2)y = \tan a x $
  \item[(d)] $ (D^2 + a^2)y = \sec 2x $
  \item[(e)] $ x^2 y'' - 4x y' + 6y = 21x^{-4} $
  \item[(f)] $ 4x^2 y'' + 8x y' - 3y = 7x^2 - 15x^3 $
  \item[(g)] $ x^2 y'' - 2x y' + 2y = x^3 \cos x $
  \item[(h)] $ x y'' - y' = (3 + x)x^2 e^x $
\end{enumerate}

\section*{10. Solve using the method of undetermined coefficients ($ D^n \equiv \frac{d^n}{dx^n} $)}

\begin{enumerate}
  \item[(a)] $ (D^3 - 2D^2 - 5D + 6)y = 18e^x $
  \item[(b)] $ (D^2 + 25)y = 50 \cos 5x + 30 \sin 5x $
  \item[(c)] $ (D^3 - 2D^2 + 4D - 8)y = 8(x^2 + \cos 2x) $
  \item[(d)] $ (D^3 + 3D^2 - 4)y = 12e^{-2x} + 9e^x $
\end{enumerate}

\section*{11.}
Show that the general solution of $ L(y) = f_1(x) + f_2(x) $, where $ L(y) $ is a linear differential operator, is $ y = \bar{y} + y^* $, where $ \bar{y} $ is the general solution of $ L(y) = 0 $ and $ y^* $ is the sum of any particular solutions of $ L(y) = f_1(x) $ and $ L(y) = f_2(x) $.

\end{document}